Review case study of control inversion.

theories/cascade.v
@@ -1,226 +1,306 @@
-(* cascade.v
+(* cascade.v *)
 
-   Verification of the program [invert], an example of control inversion using
-   effect handlers.
+(* This file contains the verification of [invert], a program that
+   applies an effect handler to transform a higher-order iteration
+   method into a lazy sequence. A higher-order iteration method is
+   a function [iter] of type [('a -> unit) -> unit]. It applies an
+   input function [f : 'a -> unit] to the elements of a collection.
+   It "consumes" the elements of this collection. A lazy sequence
+   "produces" elements. It is a thunk that, when forced, produces
+   either a pair of one element of the structure and a sequence for
+   the remaining elements, or a marker of the end of the collection.
 *)
 
-From stdpp              Require Import list.
-From iris.proofmode     Require Import base tactics classes.
-From iris.algebra       Require Import excl_auth.
+From stdpp Require Import list.
+From iris.proofmode Require Import base tactics classes.
+From iris.algebra Require Import excl_auth.
 From iris.program_logic Require Import weakestpre.
-From hazel              Require Import notation weakestpre deep_handler.
-
-Section iter.
-
-(** Folds. *)
-
-(* Specification of an iterator. *)
-
-Class IterLib Σ `{!irisGS eff_lang Σ} := {
-  iter      : val;
-  permitted : list val → iProp Σ;
-  complete  : list val → iProp Σ;
-  S         : iProp Σ;            
-  S'        : iProp Σ;
-
-  iter_spec E (I : list val → iProp Σ)
-              (Ψ : iEff Σ) (f : val) :
-
-    □ (∀ us u, permitted (us ++ [u]) -∗
-       S' -∗
-         I us -∗
-           EWP f u @ E <| Ψ |> {{ _, S' ∗ I (us ++ [u]) }}) -∗
-
-    S -∗
-      I [] -∗
-        EWP iter f @ E <| Ψ |> {{ _, ∃ xs, S ∗ I xs ∗ complete xs }};
-}.
-
-End iter.
+From hazel Require Import notation weakestpre deep_handler tactics.
 
 
-Section invert.
-Context `{!heapG Σ} {HIterLib: IterLib Σ}.
+(** Implementation. *)
 
-(** Control Invertion. *)
+(* Implementation of [invert] in HH. *)
 
-(* The program [invert] takes an iterator as input and returns a stream of the
-   elements in the underlying collection. It does so by halting the iteration
-   each time it bumps into a new element.
-*)
+Section implementation.
 
-Definition invert : val := λ: "iter",
-  let: "yield" := λ: "x", do: "x" in
-  λ: <>,
+  (* Sequences. *)
+
+  (* In OCaml, the type of sequences can be defined as follows:
+
+       type 'a seq  = unit -> 'a head
+        and 'a head = Nil | Cons of 'a * 'a seq
+
+     In HH, we encode sequences as functions from unit to binary
+     sums encoding the inhabitants of the type ['a head]:
+  *)
+
+  Definition sCons (x k : expr) : expr := SOME (x, k).
+  Definition sNil               : val  := NONEV%V.
+
+
+  (* Invert. *)
+
+  (* The program [invert] installs a handler over the application
+     of [iter] to [yield]. The function [yield] performs an effect
+     every time it is applied to an element of the collection. When
+     [yield] performs an effect with such an element [x], the effect
+     branch receives this element as well as a continuation [k]
+     representing the paused execution of [iter]. It then packages
+     both of these values into a [Cons] pair. When the iteration
+     terminates, the return branch assumes control and returns a
+     [Nil] head.
+  *)
+
+  Definition invert : val := λ: "iter", λ: <>,
+    let: "yield" := λ: "x", do: "x" in
     try: "iter" "yield" with
-      effect (λ: "u" "k", SOME ("u", "k"))%V
-    | return (λ: <>, NONEV)%V
+      effect λ: "x" "k", sCons "x" "k"
+    | return λ: <>, sNil
     end.
 
-
-(** Cascades. *)
-
-(* Definition of the predicate [cascade]. *)
-
-Definition cascade_pre :
-  (val -d> list val -d> iPropO Σ) → (val -d> list val -d> iPropO Σ)
-  := λ cascade k us,
-     EWP k #() {{ y,
-       match y with
-       | NONEV        => complete   us         ∗ S
-       | SOMEV (u, k) => permitted (us ++ [u]) ∗ ▷ cascade k (us ++ [u])
-       | _ => False
-       end }}%I.
-
-Local Instance cascade_pre_contractive : Contractive cascade_pre.
-Proof.
-  rewrite /cascade_pre => n cascade cascade' Hcascade k us.
-  f_equiv=>?. simpl.
-  repeat (f_contractive || f_equiv); try apply Hcascade.
-Qed.
-Definition cascade_def : val -d> list val -d> iPropO Σ :=
-  fixpoint (cascade_pre).
-Definition cascade_aux : seal cascade_def. Proof. by eexists. Qed.
-Definition cascade := cascade_aux.(unseal).
-Definition cascade_eq : cascade = cascade_def := cascade_aux.(seal_eq).
-Global Lemma cascade_unfold k us : cascade k us ⊣⊢ cascade_pre cascade k us.
-Proof.
-  rewrite cascade_eq /cascade_def.
-  by apply (fixpoint_unfold cascade_pre).
-Qed.
+End implementation.
 
 
-(** Protocol. *)
+(** Specification. *)
 
-(* The protocol [Ψ_seq] is used in the verification of [invert]. It describes
-   the interaction between the computation [iter yield] and its handler. *)
+(* The specification of [invert] depends on (1) the specification
+   of a iteration method and (2) the specification of a lazy sequence,
+   Both of which depend on the predicates [permitted], [complete],
+   and [canTraverse]. These predicates are tied to the implicit data
+   structure that an iteration method [iter] traverses and whose
+   elements a lazy sequence produces.
+*)
 
-Definition Ψ_seq I : iEff Σ :=
-  (>> us u >> 
-    !  u  {{ I  us         ∗ permitted (us ++ [u]) }};
-    ? #() {{ I (us ++ [u])                         }}).
+Section specification.
+
+  (* Specification of iteration methods. *)
+
+  Section iteration_methods.
+
+    Class isIter Σ `{!irisGS eff_lang Σ} := {
+      (* Program that traverses the structure. *)
+      iter : val;
+
+      (* Predicate that describes the possible partial paths. *)
+      permitted : list val → iProp Σ;
+
+      (* Predicate that describes the possible complete paths. *)
+      complete : list val → iProp Σ;
+
+      (* Permission to traverse a structure. *)
+      canTraverse : iProp Σ;
+
+      (* Specification of [iter]. *)
+      iter_spec E
+        (I : list val → iProp Σ) (* Loop invariant. *)
+        (Ψ : iEff Σ)             (* Iteratee's effects. *)
+        (f : val) :
+
+        (* "If [f] bumps [I] by one step, ..." *)
+        □ (∀ us u,
+             permitted (us ++ [u]) -∗
+               I us -∗
+                 EWP f u @ E <| Ψ |> {{ _, I (us ++ [u]) }}) -∗
+
+      (* "... then [iter f] bumps [I] by [us] steps." *)
+       canTraverse -∗
+          I [] -∗
+            EWP iter f @ E <| Ψ |>
+              {{ _, ∃ xs,
+                      I xs ∗ complete xs ∗ canTraverse
+              }};
+    }.
+
+  End iteration_methods.
+
+
+  (* Specification of lazy sequences. *)
+
+  Section lazy_sequences.
+    Context `{!heapG Σ}
+             {HisIter: isIter Σ}. (* The specification of lazy sequences
+                                     depends on the predicates [permitted],
+                                     [complete], and [canTraverse]. *)
+
+    (* Specification of heads. *)
+
+    (* The predicate [isHead] is defined as [isHead_pre isSeq],
+       where [isSeq] is the fixpoint of [isSeq_pre]. *)
+    (* A head is either a [Cons] pair or a [Nil] marker. *)
+    Definition isHead_pre
+      (isSeq :  val -d> list val -d> iPropO Σ)
+             : (val -d> list val -d> iPropO Σ) := λ h us,
+      match h with
+      | NONEV        => complete   us         ∗ canTraverse
+      | SOMEV (u, k) => permitted (us ++ [u]) ∗ ▷ isSeq k (us ++ [u])
+      | _ => False
+      end%I.
+
+    (* Specification of sequences. *)
+
+    (* A sequence is a thunk [k] that when applied to [#(0]
+       produces a head [h] s.t. [isHead h us]. *)
+    Definition isSeq_pre
+      (isSeq :  val -d> list val -d> iPropO Σ)
+             : (val -d> list val -d> iPropO Σ) := λ k us,
+      EWP k #() {{ h, isHead_pre isSeq h us }}%I.
+
+    (* [isSeq_pre] is contractive, therefore it admits a fixpoint. *)
+    Local Instance isHead_pre_contractive : Contractive isSeq_pre.
+    Proof.
+      rewrite /isSeq_pre /isHead_pre => n isSeq isSeq' HisSeq k us.
+      f_equiv=>?. simpl. by repeat (f_contractive || f_equiv).
+    Qed.
+    Definition isSeq_def : val -d> list val -d> iPropO Σ := fixpoint (isSeq_pre).
+    Definition isSeq_aux : seal isSeq_def. Proof. by eexists. Qed.
+    Definition isSeq := isSeq_aux.(unseal).
+    Definition isHead := isHead_pre isSeq.
+    Definition isSeq_eq : isSeq = isSeq_def := isSeq_aux.(seal_eq).
+    Global Lemma isSeq_unfold k us : isSeq k us ⊣⊢ isSeq_pre isSeq k us.
+    Proof. by rewrite isSeq_eq/isSeq_def;apply(fixpoint_unfold isSeq_pre). Qed.
+    Global Lemma isHead_unfold h us : isHead h us = isHead_pre isSeq h us.
+    Proof. done. Qed.
+
+  End lazy_sequences.
+
+
+  (* Specification of [invert]. *)
+
+  Section invert.
+    Context `{!heapG Σ} {HisIter: isIter Σ}.
+
+    Definition invert_spec : iProp Σ :=
+      canTraverse -∗
+        EWP invert iter <| ⊥ |> {{ k,
+          isSeq k [] }}.
+
+  End invert.
+
+End specification.
+
 
 (** Verification. *)
 
-(* Camera setup. *)
+(* The key ideas in the verification of [invert] are the
+   introduction of a piece of ghost state to describe the
+   elements seen by handler and handlee, and the application
+   of the reasoning rule for deep handlers.
+*)
 
-Context `{!inG Σ (excl_authR (leibnizO (list val)))}.
+Section verification.
 
-Definition handler_state γ us : iProp Σ := own γ (●E (us : ofe_car (leibnizO (list val)))).
-Definition  client_state γ us : iProp Σ := own γ (◯E (us : ofe_car (leibnizO (list val)))).
+  Section ghost_theory.
+    (* We use ghost variables with contents in the CMRA [Auth(Ex(List Val))]. *)
+    Context `{!inG Σ (excl_authR (leibnizO (list val)))}.
 
-(* Ghost theory. *)
+    (* The assertion [own γ (●E us)] states that the handler
+       has seen the elements [us]. *)
+    Definition handlerSt γ us : iProp Σ :=
+      own γ (●E (us : ofe_car (leibnizO (list val)))).
+    (* The assertion [own γ (◯E us)] states that [iter]
+       has seen the elements [us]. *)
+    Definition iterSt γ us : iProp Σ :=
+      own γ (◯E (us : ofe_car (leibnizO (list val)))).
 
-Lemma ghost_state_alloc us : ⊢ (|==> ∃ γ, handler_state γ us ∗ client_state γ us)%I.
-Proof.
-  iMod (own_alloc ((●E (us : ofe_car (leibnizO (list val)))) ⋅
-                   (◯E (us : ofe_car (leibnizO (list val)))))) as (γ) "[??]";
-  [ apply excl_auth_valid | eauto with iFrame ]; done.
-Qed.
-Lemma ghost_state_agree γ us vs : handler_state γ us -∗ client_state γ vs -∗ ⌜ us = vs ⌝.
-Proof.
-  iIntros "Hγ● Hγ◯".
-  by iDestruct (own_valid_2 with "Hγ● Hγ◯") as %?%excl_auth_agree_L.
-Qed.
-Lemma ghost_var_update γ ws us vs :
-  handler_state γ us -∗ client_state γ vs ==∗ handler_state γ ws  ∗ client_state γ ws.
-Proof.
-  iIntros "Hγ● Hγ◯".
-  iMod (own_update_2 _ _ _ (●E (ws : ofe_car (leibnizO (list val))) ⋅
-                            ◯E (ws : ofe_car (leibnizO (list val))))
-    with "Hγ● Hγ◯") as "[$$]";
-  [ apply excl_auth_update |]; done.
-Qed.
+    (* Create a new ghost cell from this CMRA. *)
+    (* In the verification of [invert], the ghost variable [γ]
+       initially holds the empty list. *)
+    Lemma new_cell us : ⊢ (|==> ∃ γ, handlerSt γ us ∗ iterSt γ us)%I.
+    Proof.
+      iMod (own_alloc ((●E (us : ofe_car (leibnizO (list val)))) ⋅
+                       (◯E (us : ofe_car (leibnizO (list val)))))) as (γ) "[??]";
+      [ apply excl_auth_valid | eauto with iFrame ]; done.
+    Qed.
 
-(* Correctness of the handler. *)
+    (* Handler and [iter]'s views are in agreement. *)
+    Lemma confront_views γ us vs : handlerSt γ us -∗ iterSt γ vs -∗ ⌜us = vs⌝.
+    Proof.
+      iIntros "Hγ● Hγ◯".
+      by iDestruct (own_valid_2 with "Hγ● Hγ◯") as %?%excl_auth_agree_L.
+    Qed.
 
-Lemma invert_handler E γ us :
-  handler_state γ us -∗
-    deep_handler E (λ: "u" "k", SOME ("u", "k"))%V (λ: <>, NONEV)%V
-     (* Ψ  *) (Ψ_seq (client_state γ))
-     (* Ψ' *) ⊥
-     (* Φ  *) (λ _, ∃ vs, S ∗ client_state γ vs ∗ complete vs)
-     (* Φ' *) (λ y , match y with
-               | NONEV        => complete   us         ∗ S
-               | SOMEV (u, k) => permitted (us ++ [u]) ∗ cascade k (us ++ [u])
-               | _ => False
-               end)%I.
-Proof.
-  iLöb as "IH" forall (us γ).
-  rewrite !deep_handler_unfold /deep_handler_eq.
-  iIntros "Hhstate". iSplit.
-  - iIntros (v) "HΦ". iDestruct "HΦ" as (vs) "(HS & Hcstate & Hcomplete)".
-    iDestruct (ghost_state_agree with "Hhstate Hcstate") as "<-". iNext.
-    iApply ewp_pure_step. apply pure_prim_step_beta. simpl.
-    iApply ewp_value. by iFrame.
-  - iIntros (u k) "Hhandler". iNext.
-    rewrite /(Ψ_seq (client_state γ)).
-    rewrite (protocol_agreement_tele' [tele _ _] [tele]) //=.
-    iApply fupd_ewp.
-    iDestruct "Hhandler" as (us' u') "(<- & [Hcstate Hpermitted] & Hk)".
-    iDestruct (ghost_state_agree with "Hhstate Hcstate") as "%".
-    rewrite -H. clear H.
-    iMod (ghost_var_update _ (us ++ [u]) with "Hhstate Hcstate") as "[Hhstate Hcstate]".
-    iSpecialize ("Hk" with "Hcstate"). iModIntro.
-    iApply (Ectxi_ewp_bind (AppLCtx _)). reflexivity.
-    iApply ewp_pure_step. apply pure_prim_step_beta. simpl.
-    iApply ewp_pure_step. apply pure_prim_step_rec.
-    iApply ewp_value. simpl.
-    iApply ewp_pure_step. apply pure_prim_step_beta. simpl.
-    iApply (Ectxi_ewp_bind InjRCtx). reflexivity.
-    iApply ewp_pure_step. apply pure_prim_step_pair.
-    iApply ewp_value. simpl.
-    iApply ewp_pure_step'. apply pure_prim_step_InjR.
-    iApply ewp_value. simpl. iNext.
-    rewrite !cascade_unfold /cascade_pre.
-    iFrame. iSpecialize ("IH" with "Hhstate").
-    iSpecialize ("Hk" with "IH"). iApply (ewp_strong_mono with "Hk").
-    done. iApply iEff_le_refl.
-    iIntros (v). simpl.
-    destruct v; try naive_solver.
-    destruct v; try naive_solver.
-    iIntros "[HP Hcascade]". iModIntro. by iFrame.
-Qed.
+    (* With the ownership of both views, one can update the contents of [γ]. *)
+    Lemma update_cell γ ws us vs :
+      handlerSt γ us -∗ iterSt γ vs ==∗ handlerSt γ ws  ∗ iterSt γ ws.
+    Proof.
+      iIntros "Hγ● Hγ◯".
+      iMod (own_update_2 _ _ _ (●E (ws : ofe_car (leibnizO (list val))) ⋅
+                                ◯E (ws : ofe_car (leibnizO (list val))))
+        with "Hγ● Hγ◯") as "[$$]";
+      [ apply excl_auth_update |]; done.
+    Qed.
 
-(* Spec and proof of [invert]. *)
+  End ghost_theory.
 
-Lemma invert_spec :
-  S -∗ EWP invert iter {{ k, cascade k [] }}.
-Proof.
-  iIntros "HS". unfold invert.
-  iApply fupd_ewp. iMod (ghost_state_alloc []) as (γ) "[Hhstate Hcstate]". iModIntro.
-  iApply ewp_pure_step. apply pure_prim_step_beta. simpl.
-  iApply (Ectxi_ewp_bind (AppRCtx _)). done.
-  iApply ewp_pure_step. apply pure_prim_step_rec.
-  iApply ewp_value. simpl.
-  iApply (Ectxi_ewp_bind (AppLCtx _)). done.
-  iApply ewp_pure_step. apply pure_prim_step_rec.
-  iApply ewp_value. simpl.
-  iApply ewp_pure_step. apply pure_prim_step_beta. simpl.
-  iApply ewp_pure_step. apply pure_prim_step_rec.
-  iApply ewp_value. simpl.
-  rewrite !cascade_unfold cascade_eq.
-  iApply ewp_pure_step. apply pure_prim_step_beta. simpl.
-  iApply (ewp_mono with "[HS Hhstate Hcstate]"); [|
-  iApply (ewp_deep_try_with with "[HS Hcstate]"); [|
-  iApply (invert_handler with "Hhstate") ]].
-  - iIntros (v). simpl. rewrite cascade_eq.
-    destruct v; try naive_solver.
-    destruct v; try naive_solver.
-    iIntros "[HP Hcascade]". iModIntro. by iFrame.
-  - iApply (ewp_mono with "[HS Hcstate]"); [|
-    iApply (iter_spec _ (client_state γ) (Ψ_seq _)
-               (λ: "x", do: "x")%V with "[] HS Hcstate") ].
-    + simpl. iIntros (_) "H". iModIntro.
-      iDestruct "H" as (vs) "(HS & Hcstate & Hcomplete)".
-      iExists vs. by iFrame.
-    + iModIntro. iIntros (us u) "Hpermitted HS' Hcstate".
-      iApply ewp_pure_step. apply pure_prim_step_beta. simpl.
-      iApply ewp_pure_step. apply pure_prim_step_do. simpl.
-      iApply ewp_eff. rewrite /Ψ_seq.
-      rewrite (protocol_agreement_tele' [tele _ _] [tele]) //=.
-      iExists us, u. iFrame. iSplit; [done|].
-      iIntros "Hcstate". iModIntro. iApply ewp_value. by iFrame.
-Qed.
+  Section invert_correct.
+    Context `{!heapG Σ}
+             {HisIter: isIter Σ}
+            `{!inG Σ (excl_authR (leibnizO (list val)))}.
 
-End invert.
+    (* This protocol describes the effects performed by [yield]. *)
+     Definition Ψ_yield I : iEff Σ :=
+      (>> us u >> !u   {{ I us ∗ permitted (us ++ [u]) }};
+                  ?#() {{ I (us ++ [u]) }}).
+
+    (* The [yield] handler is correct. *)
+    Lemma yield_handler_correct γ (vs : list val) :
+      handlerSt γ vs -∗
+        deep_handler ⊤ (λ: "x" "k", sCons "x" "k")%V (λ: <>, sNil)%V
+         (* Client's protocol:  *)
+           (Ψ_yield (iterSt γ))
+         (* Handler's protocol: *)
+           ⊥
+         (* Client's postcondition:  *)
+           (λ _, ∃ (us : list val), iterSt γ us ∗ complete us ∗ canTraverse)
+         (* Handler's postcondition: *)
+           (λ h , isHead h vs).
+    Proof.
+      iLöb as "IH" forall (vs γ).
+      rewrite !deep_handler_unfold /deep_handler_eq.
+      iIntros "HhandlerSt". iSplit.
+      - iIntros (v) "HΦ".
+        iDestruct "HΦ" as (us) "(HiterSt & Hcomplete & HcanTraverse)".
+        iDestruct (confront_views with "HhandlerSt HiterSt") as "<-".
+        iNext. unfold sNil. ewp_pure_steps. by iFrame.
+      - iIntros (u k) "Hhandler". iNext.
+        rewrite /(Ψ_yield (iterSt γ)).
+        rewrite (protocol_agreement_tele' [tele _ _] [tele]) //=.
+        iDestruct "Hhandler" as (us u') "(<- & [HiterSt Hpermitted] & Hk)".
+        iApply fupd_ewp.
+        iDestruct (confront_views with "HhandlerSt HiterSt") as "%Heq".
+        rewrite Heq. clear Heq.
+        iMod (update_cell _ (us ++ [u]) with "HhandlerSt HiterSt")
+          as "[HhandlerSt HiterSt]".
+        iModIntro.
+        iSpecialize ("Hk" with "HiterSt").
+        unfold sCons. ewp_pure_steps. iFrame. iNext.
+        rewrite !isSeq_unfold /isSeq_pre.
+        iSpecialize ("IH" with "HhandlerSt").
+        by iApply ("Hk" with "IH").
+    Qed.
+
+    (* [invert] is correct. *)
+    Lemma invert_correct : ⊢ invert_spec.
+    Proof.
+      iIntros "HcanTraverse". unfold invert.
+      iApply fupd_ewp.
+      iMod (new_cell []) as (γ) "[HhandlerSt HiterSt]".
+      iModIntro. ewp_pure_steps.
+      rewrite !isSeq_unfold isSeq_eq /isSeq_pre.
+      do 10 ewp_value_or_step.
+      iApply (ewp_deep_try_with with "[HcanTraverse HiterSt]").
+      - iApply (iter_spec _ (iterSt γ) (Ψ_yield (iterSt γ))
+          with "[] HcanTraverse HiterSt").
+        iModIntro. iIntros (us u) "Hpermitted HiterSt".
+        ewp_pure_steps. iApply ewp_eff. rewrite /Ψ_yield.
+        rewrite (protocol_agreement_tele' [tele _ _] [tele]) //=.
+        iExists us, u. iFrame. iSplit; [done|].
+        iIntros "HiterSt". by ewp_pure_steps.
+      - rewrite -isSeq_eq.
+        by iApply (handler_judgment with "HhandlerSt").
+    Qed.
+
+  End invert_correct.
+
+End verification.
